bedrock2/src/bedrock2/memory_mapped_ext_spec.v
@@ -10,7 +10,7 @@ Require coqutil.Datatypes.String.
 Require Import coqutil.Map.Interface coqutil.Map.Domain.
 Require Import coqutil.Word.Interface coqutil.Word.Bitwidth.
 Require Import coqutil.Word.Properties.
-Require Import bedrock2.Semantics.
+Require Import bedrock2.Semantics bedrock2.LeakageSemantics.
 Require Import bedrock2.TraceInspection.
 Local Open Scope string_scope.
 
@@ -50,16 +50,16 @@ Section WithMem.
      be compiled to a RISC-V load or store instruction *)
   Definition ext_spec{mmio_ext_calls: MemoryMappedExtCalls}: ExtSpec :=
     fun (t: trace) (mGive: mem) (action: string) (args: list word)
-        (post: mem -> list word -> Prop) =>
+        (post: mem -> list word -> list word -> Prop) =>
       exists n, (n = 1 \/ n = 2 \/ n = 4 \/ (n = 8 /\ width = 64%Z))%nat /\
       ((action = "memory_mapped_extcall_read" ++ String.of_nat (n * 8) /\
         exists addr, args = [addr] /\ mGive = map.empty /\
                      read_step n t addr (fun v mRcv =>
-                         post mRcv [word.of_Z (LittleEndian.combine n v)])) \/
+                         post mRcv [word.of_Z (LittleEndian.combine n v)] [addr])) \/
        (action = "memory_mapped_extcall_write" ++ String.of_nat (n * 8) /\
         exists addr v, args = [addr; word.of_Z (LittleEndian.combine n v)] /\
                        write_step n t addr v mGive /\
-                       post map.empty nil)).
+                       post map.empty nil [addr])).
 
   Definition footprint_list(addr: word)(n: nat): list word :=
     List.unfoldn (word.add (word.of_Z 1)) n addr.
@@ -100,7 +100,7 @@ Section WithMem.
   Lemma weaken_ext_spec{mmio_ext_calls: MemoryMappedExtCalls}
     {mmio_ext_calls_ok: MemoryMappedExtCallsOk mmio_ext_calls}:
     forall t mGive a args post1 post2,
-      (forall mRcv rets, post1 mRcv rets -> post2 mRcv rets) ->
+      (forall mRcv rets klist, post1 mRcv rets klist -> post2 mRcv rets klist) ->
       ext_spec t mGive a args post1 ->
       ext_spec t mGive a args post2.
   Proof.
